theories/Semantics/HeadTransition.v
@@ -6,7 +6,8 @@ From Coq Require Import Program Morphisms Relations.Relation_Definitions.
 From Coinduction Require Import all.
 From PTree.Core Require Import PTreeDefinition.
 From PTree.Prob Require Import TwoLevelMeasure.
-From PTree.Eq Require Import UnifiedFrontier PrimitiveStableHitting PTreeKernel PEutt.
+From PTree.Eq Require Import UnifiedFrontier PrimitiveStableHitting PTreeKernel
+  StableHittingRelation.
 
 Set Implicit Arguments.
 Unset Strict Implicit.
